En utilisant les produits matriciels on montre que   \vspace{4pt}
% \begin{multicols}{1}
    \begin{enumerate}[a)]
        \item $\hat{H}\hat{X}\hat{H} = \hat{Z}$
        \begin{align*}
            \frac{1}{\sqrt{2}}\pmqty{1 & 1 \\ 1 & -1}\pmqty{0 & 1 \\ 1 & 0}\frac{1}{\sqrt{2}}\pmqty{1 & 1 \\ 1 & -1} = \frac{1}{2}\pmqty{2 & 0 \\ 0 & -2} = \hat{Z}
        \end{align*}
        \item $\hat{S}\hat{X}\hat{S}^\dagger = \hat{Y}$
        \begin{align*}
            \pmqty{1 & 0 \\ 0 & i}\pmqty{0 & 1 \\ 1 & 0}\pmqty{1 & 0 \\ 0 & -i} = \pmqty{0 & -i \\ i & 0} = \hat{Y}
        \end{align*}
        \item $\hat{S}\hat{Z}\hat{S}^\dagger = \hat{Z}$
        \begin{align*}
            \pmqty{1 & 0 \\ 0 & i}\pmqty{1 & 0 \\ 0 & -1}\pmqty{1 & 0 \\ 0 & -i} = \pmqty{1 & 0 \\ 0 & -1} = \hat{Z}
        \end{align*}
        \item $\hat{X}\hat{Z}\hat{X} = -\hat{Z}$
        \begin{align*}
            \pmqty{0 & 1 \\ 1 & 0} \pmqty{1 & 0 \\ 0 & -1} \pmqty{0 & 1 \\ 1 & 0} = \pmqty{-1 & 0 \\ 0 & 1} = -\hat{Z}
        \end{align*}
    \end{enumerate}
% \end{multicols}